fsFFI: add 1 parameter to #write and done with specs

basis/fsioProgScript.sml
@@ -3,7 +3,6 @@ open preamble
      cfTacticsBaseLib cfTacticsLib basisFunctionsLib
      mlstringTheory mlcommandLineProgTheory fsFFITheory
 
-
 val _ = new_theory"fsioProg";
 val _ = translation_extends "mlcommandLineProg";
 
@@ -19,10 +18,10 @@ val _ = process_topdecs `
 ` |> append_prog
 
 (* 257 w8 array *)
-val buff257_e = ``(App Aw8alloc [Lit (IntLit 257); Lit (Word8 0w)])``
+val iobuff_e = ``(App Aw8alloc [Lit (IntLit 257); Lit (Word8 0w)])``
 val _ = ml_prog_update
-          (add_Dlet (derive_eval_thm "buff257_loc" buff257_e) "buff257" [])
-val buff257_loc_def = definition "buff257_loc_def"
+          (add_Dlet (derive_eval_thm "iobuff_loc" iobuff_e) "iobuff" [])
+val iobuff_loc_def = definition "iobuff_loc_def"
 
 (* stdin, stdout, stderr *)
 (* these are functions as append_prog rejects constants *)
@@ -31,41 +30,38 @@ val _ = process_topdecs`
     fun stdout () = Word8.fromInt 1;
     fun stderr () = Word8.fromInt  2
     ` |> append_prog
- (* 
-    process_topdecs` val stdtest = Word8.fromInt 0 ` |> append_dec
-*)
 
-(* higher-lever write function which calls #write until something is written or
+(* writei: higher-lever write function which calls #write until something is written or
 * an filesystem error is raised and outputs the number of bytes written.
-* It assumes that buff257 is initialised *)
+* It assumes that iobuff is initialised 
+* write: idem, but keeps writing until the whole (specified part of the) buffer
+* is written *)
 
 val _ =
   process_topdecs`fun writei fd n i =
-    let val a = Word8Array.update buff257 0 fd
-        val a = Word8Array.update buff257 1 n
-        val a = Word8Array.update buff257 2 i
-        val a = #(write) buff257 in
-        if Word8Array.sub buff257 0 = Word8.fromInt 1 
+    let val a = Word8Array.update iobuff 0 fd
+        val a = Word8Array.update iobuff 1 n
+        val a = Word8Array.update iobuff 2 i
+        val a = #(write) iobuff in
+        if Word8Array.sub iobuff 0 = Word8.fromInt 1 
         then raise InvalidFD
         else 
-          let val nw = Word8.toInt(Word8Array.sub buff257 1) in
+          let val nw = Word8.toInt(Word8Array.sub iobuff 1) in
             if nw = 0 then writei fd n i
             else nw
           end
     end
     fun write fd n i = 
-    let val nw = writei fd n i in
-      if nw < n then write fd (n-nw) (i+nw) else () end` |> append_prog
+      if n = 0 then () else
+        let val nw = writei fd (Word8.fromInt n) (Word8.fromInt i) in
+          if nw < n then write fd (n-nw) (i+nw) else () end` |> append_prog
 
 
 
 (* Output functions on given file descriptor *)
 val _ = 
   process_topdecs` fun write_char fd c = 
-    let val a = Word8Array.update buff257 2 (Word8.fromInt(Char.ord c))
-        val i = Word8.fromInt 1
-        val r = write fd i
-    in () end
+    (Word8Array.update iobuff 3 (Word8.fromInt(Char.ord c)); write fd 1 0; ())
 
     fun print_char c = write_char (stdout()) c
     fun prerr_char c = write_char (stderr()) c
@@ -104,10 +100,11 @@ val _ = process_topdecs
 val _ = 
   process_topdecs` fun write_string fd s =
   if s = "" then () else
-  let val s1 = String.substring s 0 254
-      val fl = copyi buff257 2 (String.explode s1)
-      val nw = write fd (Word8.fromInt(String.strlen s1)) in
-         write_string fd (String.extract s nw NONE)
+  let val s1 = String.substring s 0 255
+      val fl = copyi iobuff 3 (String.explode s1)
+      val n = String.strlen s1
+      val a = write fd n 0 in
+         write_string fd (String.extract s n NONE)
   end` |> append_prog
 
 (* val print_newline : unit -> unit *)
@@ -127,37 +124,38 @@ val _ = process_topdecs
 
 val _ = process_topdecs`
 fun open_in fname =
-  let val a = str_to_w8array buff257 fname
-      val a = #(open_in) buff257 in
-        if Word8Array.sub buff257 0 = Word8.fromInt 0 
-        then Word8Array.sub buff257 1
+  let val a = str_to_w8array iobuff fname
+      val a = #(open_in) iobuff in
+        if Word8Array.sub iobuff 0 = Word8.fromInt 0 
+        then Word8Array.sub iobuff 1
         else raise BadFileName
   end
 fun open_out fname =
-  let val a = str_to_w8array buff257 fname
-      val a = #(open_out) buff257 in
-        if Word8Array.sub buff257 0 = Word8.fromInt 0 
-        then Word8Array.sub buff257 1
+  let val a = str_to_w8array iobuff fname
+      val a = #(open_out) iobuff in
+        if Word8Array.sub iobuff 0 = Word8.fromInt 0 
+        then Word8Array.sub iobuff 1
         else raise BadFileName
   end` |> append_prog
 
 (* val input : in_channel -> bytes -> int -> int -> int
 * input ic buf pos len reads up to len characters from the given channel ic,
 * storing them in byte sequence buf, starting at character number pos. *)
+(* TODO: rewrite with read *)
 val _ = 
   process_topdecs`
 fun input fd buf pos len =
-  let val a = Word8Array.update buff257 0 fd
+  let val a = Word8Array.update iobuff 0 fd
       fun input_aux pos len count =
-      let val a = Word8Array.update buff257 1 (min len 255)
-        val a = #(read) buff257
-        val res = Word8.toInt (Word8Array.sub buff257 0)
-        val nread = Word8.toInt (Word8Array.sub buff257 1)
+      let val a = Word8Array.update iobuff 1 (min len 255)
+        val a = #(read) iobuff
+        val res = Word8.toInt (Word8Array.sub iobuff 0)
+        val nread = Word8.toInt (Word8Array.sub iobuff 1)
       in           
         if res = 1 then raise InvalidFD
         else if nread = 0 then count
         else 
-          let val a = Word8Array.copy_aux buff257 buf pos nread 2 in
+          let val a = Word8Array.copy_aux iobuff buf pos nread 2 in
             if nread < len then input_aux (pos + nread) (len - nread) count
             else (count + nread)
           end
@@ -168,18 +166,18 @@ fun input fd buf pos len =
 (* wrapper for ffi call *)
 val _ = process_topdecs`
   fun read fd n =     
-    let val a = Word8Array.update buff257 0 fd
-        val a = Word8Array.update buff257 1 n in
-          #(read) buff257
+    let val a = Word8Array.update iobuff 0 fd
+        val a = Word8Array.update iobuff 1 n in
+          #(read) iobuff
     end` |> append_prog
 
 (* reads 1 char *)
 val _ = process_topdecs`
 fun read_char fd =
   let val a = read fd (Word8.fromInt 1) in
-    if Word8.toInt (Word8Array.sub buff257 0) = 1 then raise InvalidFD
-    else if Word8.toInt (Word8Array.sub buff257 1) = 0 then raise EndOfFile
-    else Word8Array.sub buff257 2
+    if Word8.toInt (Word8Array.sub iobuff 0) = 1 then raise InvalidFD
+    else if Word8.toInt (Word8Array.sub iobuff 1) = 0 then raise EndOfFile
+    else Word8Array.sub iobuff 2
   end` |> append_prog
 
 
