basis/fsioProofScript.sml
@@ -9,19 +9,19 @@ val _ = new_theory"fsioProof";
 
 val _ = translation_extends "fsioProg";
 val _ = monadsyntax.add_monadsyntax();
-val IOFS_buff257_def = Define`
-  IOFS_buff257 =
-    SEP_EXISTS v. W8ARRAY buff257_loc v * cond (LENGTH v = 257)
+val IOFS_iobuff_def = Define`
+  IOFS_iobuff =
+    SEP_EXISTS v. W8ARRAY iobuff_loc v * cond (LENGTH v = 258)
 `;
 
 val IOFS_def = Define `
   IOFS fs = IOx fs_ffi_part fs * &(wfFS fs)`
 
-val buff257_loc = EVAL``buff257_loc`` |> curry save_thm "buff257_loc"
+val iobuff_loc = EVAL``iobuff_loc`` |> curry save_thm "iobuff_loc"
 
-val _ = export_rewrites["buff257_loc"]
+val _ = export_rewrites["iobuff_loc"]
 
-val IOFS_buff257_HPROP_INJ = Q.store_thm("IOFS_buff257_HPROP_INJ[hprop_inj]",
+val IOFS_iobuff_HPROP_INJ = Q.store_thm("IOFS_iobuff_HPROP_INJ[hprop_inj]",
 `!fs1 fs2. HPROP_INJ (IOFS fs1) (IOFS fs2) (fs2 = fs1)`,
   rw[HPROP_INJ_def, IOFS_def, GSYM STAR_ASSOC, SEP_CLAUSES, SEP_EXISTS_THM,
      HCOND_EXTRACT] >>
@@ -87,6 +87,12 @@ val STRING_FILENAME_UNICITY_L =
   `!f f' fv. STRING_TYPE f fv ==>
     (FILENAME f' fv <=> f' = f /\ ¬MEM #"\^@" (explode f) /\ strlen f < 256)`, 
   filename_tac);
+
+val fsupdate_unchanged = Q.store_thm("fsupdate_unchanged",
+ `get_file_content fs fd = SOME(content, pos) ==> validFD fd fs ==>
+    fsupdate fs fd 0 pos content = fs`,
+    fs[fsupdate_def,get_file_content_def,validFD_def,IO_fs_component_equality]>>
+    rw[] >> pairarg_tac >> fs[ALIST_FUPDKEY_unchanged] >> rw[]);
 
 val basis_st = get_ml_prog_state;
 (* TODO: move copy/str_to_w8array elsewhere? *)
@@ -164,7 +170,7 @@ val openIn_spec = Q.store_thm(
      CARD (FDOM (alist_to_fmap fs.infds)) < 255 ⇒
      app (p:'ffi ffi_proj) ^(fetch_v "IO.open_in" (basis_st()))
        [sv]
-       (IOFS fs * IOFS_buff257)
+       (IOFS fs * IOFS_iobuff)
        (POST
           (\wv. &(WORD (n2w (nextFD fs) :word8) wv ∧
                   validFD (nextFD fs) (openFileFS s fs 0) ∧
@@ -172,11 +178,11 @@ val openIn_spec = Q.store_thm(
                 IOFS (openFileFS s fs 0))
           (\e. &(BadFileName_exn e ∧ ~inFS_fname fs s) * IOFS fs))`,
   xcf "IO.open_in" (basis_st()) >>
-  fs[FILENAME_def, strlen_def, IOFS_def, IOFS_buff257_def] >> 
+  fs[FILENAME_def, strlen_def, IOFS_def, IOFS_iobuff_def] >> 
   xpull >>
   rename [`W8ARRAY _ fnm0`] >>
   qmatch_goalsub_abbrev_tac`catfs fs` >>
-  fs[buff257_loc_def] >>
+  fs[iobuff_loc_def] >>
   xlet_auto
   >- (xsimpl >> Cases_on`s` \\ fs[]) >>
   qabbrev_tac `fnm = insert_atI (MAP (n2w o ORD) (explode s) ++ [0w]) 0 fnm0` >>
@@ -186,10 +192,10 @@ val openIn_spec = Q.store_thm(
     xlet `POSTv u2.
             &(UNIT_TYPE () u2 /\ nextFD fs < 255 /\
               validFD (nextFD fs) (openFileFS s fs 0)) *
-            W8ARRAY buff257_loc (LUPDATE 0w 0 (LUPDATE (n2w (nextFD fs)) 1 fnm)) *
+            W8ARRAY iobuff_loc (LUPDATE 0w 0 (LUPDATE (n2w (nextFD fs)) 1 fnm)) *
             catfs fs'`
     >- (simp[Abbr`catfs`,Abbr`fs'`] >>
-        xffi >> simp[fsioProgTheory.buff257_loc_def] >>
+        xffi >> simp[fsioProgTheory.iobuff_loc_def] >>
         simp[fsFFITheory.fs_ffi_part_def,IOx_def] >>
         qmatch_goalsub_abbrev_tac`IO st f ns` >>
         CONV_TAC(RESORT_EXISTS_CONV List.rev) >>
@@ -206,13 +212,13 @@ val openIn_spec = Q.store_thm(
         csimp[nextFD_ltX, openFileFS_def, openFile_def, validFD_def]) >>
     xlet_auto
     >- (xsimpl >> csimp[HD_LUPDATE] >> simp[Abbr`fnm`, LENGTH_insert_atI, LENGTH_explode]) >>
-    fs[buff257_loc_def] >>
+    fs[iobuff_loc_def] >>
     xlet_auto
-    >- (xsimpl >> rw[Abbr`fnm`,LENGTH_insert_atI,LENGTH_explode,buff257_loc,HD_LUPDATE]) >>
+    >- (xsimpl >> rw[Abbr`fnm`,LENGTH_insert_atI,LENGTH_explode,iobuff_loc,HD_LUPDATE]) >>
     xlet_auto >- (xsimpl) >>
     xif
     >-(
-       xapp >> simp[fsioProgTheory.buff257_loc_def] >> xsimpl >>
+       xapp >> simp[fsioProgTheory.iobuff_loc_def] >> xsimpl >>
     fs[EL_LUPDATE,Abbr`fnm`,LENGTH_insert_atI,LENGTH_explode,wfFS_openFile,Abbr`fs'`]) >>
     xlet_auto
     >- (xcon >> xsimpl)
@@ -228,9 +234,9 @@ val openIn_spec = Q.store_thm(
   ) >>
   xlet `POSTv u2.
             &UNIT_TYPE () u2 * catfs fs *
-            W8ARRAY buff257_loc (LUPDATE 255w 0 fnm)`
+            W8ARRAY iobuff_loc (LUPDATE 255w 0 fnm)`
   >- (
-      simp[Abbr`catfs`,Abbr`fs'`] >> xffi >> simp[buff257_loc_def] >>
+      simp[Abbr`catfs`,Abbr`fs'`] >> xffi >> simp[iobuff_loc_def] >>
       simp[fsFFITheory.fs_ffi_part_def,IOx_def] >>
       qmatch_goalsub_abbrev_tac`IO st f ns` >>
       CONV_TAC(RESORT_EXISTS_CONV List.rev) >>
@@ -242,7 +248,7 @@ val openIn_spec = Q.store_thm(
 	   implode_explode, LENGTH_explode] >>
       simp[not_inFS_fname_openFile]) >>      
   xlet_auto >-(xsimpl) >>
-  fs[buff257_loc] >>
+  fs[iobuff_loc] >>
   xlet_auto
   >- (xsimpl >> csimp[HD_LUPDATE] >> simp[Abbr`fnm`, LENGTH_insert_atI, LENGTH_explode]) >>
   xlet_auto >-(xsimpl) >>
@@ -352,45 +358,43 @@ val fsupdate_LTL = Q.store_thm("fsupdate_LTL",
    fsupdate (fs with numchars := t) fd k p c`,
    rw[] >> fs[fsupdate_def,LDROP]);
 
-val writei_spec = Q.store_thm("write_spec",
- `liveFS fs ⇒ wfFS fs ⇒ validFD (w2n fd) fs ⇒ 0 < w2n n ⇒
-  w2n fd < 255 ⇒ LENGTH rest = 255 ⇒ w2n i + w2n n <= 255
+val writei_spec = Q.store_thm("writei_spec",
+ `liveFS fs ⇒ wfFS fs ⇒ validFD (w2n fd) fs ⇒ 0 < n ⇒
+  w2n fd < 255 ⇒ LENGTH rest = 255 ⇒ i + n <= 255 ⇒
   get_file_content fs (w2n fd) = SOME(content, pos) ⇒
-  WORD (fd:word8) fdv ⇒ WORD (n:word8) nv ⇒ WORD (i:word8) iv ⇒
+  WORD (fd:word8) fdv ⇒ WORD (n2w n:word8) nv ⇒ WORD (n2w i:word8) iv ⇒
   bc = h1 :: h2 :: h3 :: rest ⇒ 
   app (p:'ffi ffi_proj) ^(fetch_v "IO.writei" (basis_st())) [fdv;nv;iv]
-  (IOFS fs * W8ARRAY buff257_loc bc) 
+  (IOFS fs * W8ARRAY iobuff_loc bc) 
   (POST
-    (\nwv. SEP_EXISTS nw. &(NUM nw nwv) * &(nw > 0) * &(nw <= w2n n) *
-           W8ARRAY buff257_loc (0w :: n2w nw :: n2w i :: rest) *
+    (\nwv. SEP_EXISTS nw. &(NUM nw nwv) * &(nw > 0) * &(nw <= n) *
+           W8ARRAY iobuff_loc (0w :: n2w nw :: n2w i :: rest) *
            IOFS(fsupdate fs (w2n fd) (1 + Lnext_pos fs.numchars) (pos + nw)
-                         (insert_atI (TAKE nw (MAP (CHR o w2n) (DROP (w2n i) rest)) pos
-                                    content))
-                                    
-                                    )
-    (\e. &(InvalidFD_exn e) * W8ARRAY buff257_loc (1w::n::rest) * &(F) *
+                         (insert_atI (TAKE nw (MAP (CHR o w2n) (DROP i rest))) pos
+                                    content)))
+    (\e. &(InvalidFD_exn e) * W8ARRAY iobuff_loc (1w:: n2w n::rest) * &(F) *
          IOFS (fs with numchars:= THE(LDROP (1 + Lnext_pos fs.numchars) fs.numchars))))`,
   strip_tac >> fs[liveFS_def] >> `?ll. fs.numchars = ll` by simp[]  >> fs[] >>
   `liveFS fs` by fs[liveFS_def] >> FIRST_X_ASSUM MP_TAC >> FIRST_X_ASSUM MP_TAC >> 
-  qid_spec_tac `bc`>> qid_spec_tac `h2` >> qid_spec_tac `h1` >> 
+  qid_spec_tac `bc`>> qid_spec_tac `h3` >>  qid_spec_tac `h2` >> qid_spec_tac `h1` >> 
   qid_spec_tac `fs` >> FIRST_X_ASSUM MP_TAC >> qid_spec_tac `ll` >> 
   HO_MATCH_MP_TAC always_eventually_ind >>
-  xcf "IO.writei" (basis_st()) >> fs[buff257_loc_def]>>
+  xcf "IO.writei" (basis_st()) >> fs[iobuff_loc_def]>>
   `ll = fs.numchars` by simp[] >> fs[]
 (* next el is <> 0 *)
   >-(sg`Lnext_pos fs.numchars = 0`   
      >-(fs[Lnext_pos_def,Once Lnext_def,liveFS_def,always_thm] >>
         cases_on`fs.numchars` >> fs[]) >>
-     NTAC 2 (xlet_auto >-(simp[LUPDATE_def] >> xsimpl)) >>
+     NTAC 3 (xlet_auto >-(simp[LUPDATE_def] >> xsimpl)) >>
      xlet`POSTv uv. &(UNIT_TYPE () uv) *
-            W8ARRAY buff257_loc (0w:: (n2w (MIN (w2n n) k)) ::rest) *
-            IOFS (fsupdate fs (w2n fd) 1 (MIN (w2n n) k + pos)
+            W8ARRAY iobuff_loc (0w:: n2w (MIN n k) :: n2w i :: rest) *
+            IOFS (fsupdate fs (w2n fd) 1 (MIN n k + pos)
                           (TAKE pos content ++ 
-                           TAKE (MIN (w2n n) k) (MAP (CHR o w2n) rest) ++ 
-                           DROP (MIN (w2n n) k + pos) content))`
+                           TAKE (MIN n k) (MAP (CHR o w2n) (DROP i rest)) ++ 
+                           DROP (MIN n k + pos) content))`
      >-(qmatch_goalsub_abbrev_tac` _ * _ * IOFS fs'` >>
         xffi >> xsimpl >>
-        fs[buff257_loc,IOFS_def,IOx_def,fs_ffi_part_def,
+        fs[iobuff_loc,IOFS_def,IOx_def,fs_ffi_part_def,
                mk_ffi_next_def] >>
         qmatch_goalsub_abbrev_tac`IO st f ns` >>
         CONV_TAC(RESORT_EXISTS_CONV List.rev) >>
@@ -405,36 +409,30 @@ val writei_spec = Q.store_thm("write_spec",
         `MEM (w2n fd) (MAP FST fs.infds)` by (metis_tac[MEM_MAP]) >>
         rw[] >> TRY(metis_tac[wfFS_fsupdate]) >>
         EVAL_TAC >>
-        (* TODO: automate? *)
-        qexists_tac`(0w::n2w (MIN (w2n n) k)::rest,fs')` >> fs[] >>
-        qexists_tac`(MIN (w2n n) k, fs')` >> fs[Abbr`fs'`,fsupdate_def] >>
+        qmatch_goalsub_abbrev_tac`_ /\ _ = SOME(xx, _ yy)` >>
+        qexists_tac`(xx,yy)` >> xsimpl >> fs[Abbr`xx`,Abbr`yy`] >>
+        qexists_tac`(MIN n k, fs')` >> xsimpl >>
         qexists_tac`(fnm, off)` >> fs[] >> rfs[] >>
-        cases_on`fs.numchars` >> fs[]) >>
+        cases_on`fs.numchars` >> fs[Abbr`fs'`,fsupdate_def]) >>
      qmatch_goalsub_abbrev_tac` _ * IOFS fs'` >>
-     qmatch_goalsub_abbrev_tac`W8ARRAY _ (_::m::rest)` >>
-     fs[buff257_loc_def] >>
-     xlet_auto >- xsimpl >>
-     xlet_auto >-(xsimpl) >>
-     fs[buff257_loc_def] >>
-     xlet_auto >- xsimpl >>
+     qmatch_goalsub_abbrev_tac`W8ARRAY _ (_::m:: n2w i :: rest)` >>
+     fs[iobuff_loc_def] >>
+     NTAC 3 (xlet_auto >- xsimpl) >>
      xif >> fs[FALSE_def] >> instantiate >>
-     xlet_auto >-(xsimpl) >>
-     fs[buff257_loc_def] >>
-     NTAC 2 (xlet_auto >- xsimpl) >>
-     `w2n n <> 0` by (cases_on`w2n n` >> fs[]) >>
+     NTAC 3 (xlet_auto >- xsimpl) >>
      xif >> fs[FALSE_def] >> instantiate >> xvar >> xsimpl >>
      instantiate >> fs[Abbr`fs'`,MIN_DEF,insert_atI_def] >> xsimpl) >>
  (* next element is 0 *)
   cases_on`fs.numchars` >- fs[liveFS_def] >> fs[] >>
-  NTAC 2 (xlet_auto >- xsimpl) >>
-  xlet`POSTv uv. &(UNIT_TYPE () uv) * W8ARRAY buff257_loc (0w:: 0w ::rest) *
+  NTAC 3 (xlet_auto >- xsimpl) >>
+  xlet`POSTv uv. &(UNIT_TYPE () uv) * W8ARRAY iobuff_loc (0w:: 0w :: n2w i :: rest) *
         IOFS (fsupdate fs (w2n fd) 1 pos
                           (TAKE pos content ++ 
-                           TAKE 0 (MAP (CHR o w2n) rest) ++ 
+                           TAKE 0 (MAP (CHR o w2n) (DROP i rest)) ++ 
                            DROP pos content))`
   >-(qmatch_goalsub_abbrev_tac` _ * _ * IOFS fs'` >>
     xffi >> xsimpl >>
-    fs[buff257_loc,IOFS_def,IOx_def,fs_ffi_part_def,
+    fs[iobuff_loc,IOFS_def,IOx_def,fs_ffi_part_def,
            mk_ffi_next_def] >>
     qmatch_goalsub_abbrev_tac`IO st f ns` >>
     CONV_TAC(RESORT_EXISTS_CONV List.rev) >>
@@ -449,10 +447,9 @@ val writei_spec = Q.store_thm("write_spec",
     `MEM (w2n fd) (MAP FST fs.infds)` by (metis_tac[MEM_MAP]) >>
     rw[] >> TRY(metis_tac[wfFS_fsupdate]) >>
     EVAL_TAC >>
-    qexists_tac`(0w::0w::rest,fs')` >> fs[] >>
+    qexists_tac`(0w::0w::n2w i::rest,fs')` >> fs[] >>
     qexists_tac`(0, fs')` >> fs[Abbr`fs'`,fsupdate_def] >>
-    qexists_tac`(fnm, off)` >> fs[] >> rfs[] >>
-    cases_on`fs.numchars` >> fs[liveFS_def]) >>
+    qexists_tac`(fnm, off)` >> fs[] >> rfs[]) >>
   NTAC 3 (xlet_auto >- xsimpl) >>
   xif >> fs[FALSE_def] >> instantiate >>
   NTAC 3 (xlet_auto >- xsimpl) >>
@@ -475,6 +472,76 @@ val writei_spec = Q.store_thm("write_spec",
     (fs[Lnext_pos_def,Once Lnext_def,liveFS_def]) >>
   fs[ADD] >> xsimpl);
 
+val fsupdate_o = Q.store_thm("fsupdate_o",
+ `validFD fd fs ==> liveFS fs ==>
+  fsupdate (fsupdate fs fd k1 pos1 c1) fd k2 pos2 c2 = 
+  fsupdate fs fd (k1+k2) pos2 c2`,
+  rw[fsupdate_def,validFD_def]
+  >-(fs[ALIST_FUPDKEY_ALOOKUP] >>
+     CASE_TAC >> fs[ALOOKUP_NONE,ALIST_FUPDKEY_o,ALIST_FUPDKEY_eq])
+  >-(fs[ALIST_FUPDKEY_o] >> HO_MATCH_MP_TAC ALIST_FUPDKEY_eq >>
+	 rw[] >> cases_on`v` >> fs[]) >>
+  fs[LDROP_ADD,liveFS_def] >>
+  imp_res_tac always_NOT_LFINITE >> imp_res_tac NOT_LFINITE_DROP >>
+  FIRST_X_ASSUM(ASSUME_TAC o Q.SPEC`k1`) >> fs[]);
+
+val insert_atI_insert_atI = Q.store_thm("insert_atI_insert_atI",
+  `pos2 = pos1 + LENGTH c1 ==>
+    insert_atI c2 pos2 (insert_atI c1 pos1 l) = insert_atI (c1 ++ c2) pos1 l`,
+    rw[insert_atI_def,TAKE_SUM,TAKE_APPEND,LENGTH_TAKE_EQ,LENGTH_DROP,
+       GSYM DROP_DROP_T,DROP_LENGTH_TOO_LONG,DROP_LENGTH_NIL_rwt]
+    >> fs[DROP_LENGTH_NIL_rwt,LENGTH_TAKE,DROP_APPEND1,TAKE_APPEND,TAKE_TAKE,
+       DROP_DROP_T,DROP_APPEND2,TAKE_LENGTH_TOO_LONG,TAKE_SUM,LENGTH_DROP]);
+
+
+val write_spec = Q.store_thm("write_spec",
+ `!n fs i pos h1 h2 h3 rest bc fdv nv iv fd content.
+  liveFS fs ⇒ wfFS fs ⇒ validFD (w2n fd) fs ⇒
+  w2n fd < 255 ⇒ LENGTH rest = 255 ⇒ i + n <= 255 ⇒
+  get_file_content fs (w2n fd) = SOME(content, pos) ⇒
+  WORD (fd:word8) fdv ⇒ NUM n nv ⇒ NUM i iv ⇒
+  bc = h1 :: h2 :: h3 :: rest ⇒ 
+  app (p:'ffi ffi_proj) ^(fetch_v "IO.write" (basis_st())) [fdv;nv;iv]
+  (IOFS fs * W8ARRAY iobuff_loc bc) 
+  (POSTv nwv. SEP_EXISTS k. IOFS_iobuff *
+     IOFS(fsupdate fs (w2n fd) k (pos + n)
+                   (insert_atI (TAKE n (MAP (CHR o w2n) (DROP i rest))) pos
+                                    content)))`,
+  strip_tac >>
+  `?N. n <= N` by (qexists_tac`n` >> fs[]) >>
+  FIRST_X_ASSUM MP_TAC >> qid_spec_tac`n` >>
+  Induct_on`N` >>
+  xcf "IO.write" (basis_st())
+  >>(xlet_auto >- xsimpl >> xif
+	 >-(TRY instantiate >> xcon >>
+		simp[IOFS_iobuff_def] >> xsimpl >> qexists_tac`0` >>
+	    fs[fsupdate_unchanged,insert_atI_def] >> xsimpl)) >>
+  NTAC 2 (xlet_auto >- xsimpl) >>
+  PURE_REWRITE_TAC[GSYM iobuff_loc_def] >>
+  xlet_auto >> xsimpl
+  >-(simp[iobuff_loc_def] >> xsimpl >> rw[] >> instantiate >> xsimpl) >> 
+  xlet_auto >- xsimpl >> reverse xif
+  >-(xcon >> xsimpl >> fs[IOFS_iobuff_def] >> xsimpl >>
+	 qexists_tac`(Lnext_pos fs.numchars + 1)` >> `nw = n` by fs[] >> xsimpl) >>
+  NTAC 2 (xlet_auto >- xsimpl) >>
+  qmatch_goalsub_abbrev_tac`IOFS fs'` >>
+  `n - nw<= N` by fs[] >>
+  FIRST_X_ASSUM (ASSUME_TAC o Q.SPECL[`n-nw`]) >> rfs[] >>
+  FIRST_X_ASSUM(ASSUME_TAC o Q.SPECL[`fs'`,`nw + i`,`pos+nw`]) >>
+  FIRST_X_ASSUM xapp_spec >> xsimpl >> instantiate >>
+  qexists_tac`insert_atI (TAKE nw (MAP (CHR ∘ w2n) (DROP i rest))) pos content` >>
+  NTAC 4 (strip_tac >-(
+		  fs[Abbr`fs'`,liveFS_def,LDROP_1, wfFS_fsupdate,validFD_def,
+			 always_DROP,ALIST_FUPDKEY_ALOOKUP,get_file_content_def,wfFS_fsupdate] >>
+		  pairarg_tac >> fs[fsupdate_def,always_DROP,ALIST_FUPDKEY_ALOOKUP])) >>
+  rw[] >> qexists_tac`Lnext_pos fs.numchars + 1 + x` >> 
+  fs[fsupdate_o,Abbr`fs'`,insert_atI_insert_atI] >>
+  qmatch_abbrev_tac`_ (_ _ _ _ _ (_ c1 _ _)) ==>> _ (_ _ _ _ _ (_ c2 _ _)) * _` >>
+  `c1 = c2` suffices_by xsimpl >> fs[Abbr`c1`,Abbr`c2`] >>
+  PURE_REWRITE_TAC[Once (Q.SPECL [`i`,`nw`] ADD_COMM)] >>
+  fs[Once ADD_COMM,GSYM DROP_DROP_T,take_drop_partition,MAP_DROP]);
+
+
 val write_char_spec = Q.store_thm("write_char_spec",
   `!(fd :word8) fdv c cv bc content pos.
     liveFS fs ⇒ wfFS fs ⇒
@@ -482,47 +549,72 @@ val write_char_spec = Q.store_thm("write_char_spec",
     get_file_content fs (w2n fd) = SOME(content, pos) ⇒
     CHAR c cv ⇒ WORD fd fdv ⇒
     app (p:'ffi ffi_proj) ^(fetch_v "IO.write_char" (basis_st())) [fdv; cv]
-    (IOFS fs * IOFS_buff257) 
-    (POST (\uv. &UNIT_TYPE () uv * IOFS_buff257 *
-                IOFS (fsupdate fs (w2n fd) (1 + Lnext_pos fs.numchars) (pos + 1)
-                     (insert_atI [c] pos content)))
-          (\e. &(InvalidFD_exn e) * &F * 
-               SEP_EXISTS rest. WORD8_ARRAY buff257_loc ((1w: word8)::1w:: 0w ::: rest) * 
-               IOFS(fs with numchars :=
-                      THE (LDROP (1 + Lnext_pos fs.numchars) fs.numchars))))`,
-  xcf "IO.write_char" (basis_st()) >> fs[IOFS_buff257_def] >> 
+    (IOFS fs * IOFS_iobuff) 
+    (POSTv uv. 
+      &UNIT_TYPE () uv * IOFS_iobuff * SEP_EXISTS k.
+      IOFS (fsupdate fs (w2n fd) k (pos+1) (insert_atI [c] pos content)))`,
+  xcf "IO.write_char" (basis_st()) >> fs[IOFS_iobuff_def] >> 
   xpull >> rename [`W8ARRAY _ bdef`] >>
-  NTAC 4 (xlet_auto >- xsimpl) >>
+  NTAC 3 (xlet_auto >- xsimpl) >>
   Cases_on `bdef` >> fs[] >> qmatch_goalsub_abbrev_tac`h1 :: t` >>
   Cases_on `t` >> fs[] >> qmatch_goalsub_abbrev_tac`h1 :: h2 :: t'` >>
-  Cases_on `t'` >> fs[] >> qmatch_goalsub_abbrev_tac`h1 :: h2 :: h3 :: rest` >>
-  simp[EVAL ``LUPDATE rr 2 (zz :: tt)``,
-       EVAL ``LUPDATE rr 1 (zz :: tt)``, LUPDATE_def] >>
-
-  PURE_REWRITE_TAC[GSYM buff257_loc_def] >>
+  Cases_on `t'` >> fs[] >> qmatch_goalsub_abbrev_tac`h1 :: h2 :: h3 :: rest'` >>
+  Cases_on `rest'` >> fs[] >> qmatch_goalsub_abbrev_tac`h1::h2::h3::h4::rest` >>
+  simp[EVAL ``LUPDATE rr 2 (zz :: tt)``, EVAL ``LUPDATE rr 1 (zz :: tt)``,
+       EVAL ``LUPDATE rr 3 (uu :: zz :: tt)``, LUPDATE_def] >>
+  PURE_REWRITE_TAC[GSYM iobuff_loc_def] >>
   xlet_auto
-  >-(PURE_REWRITE_TAC[GSYM buff257_loc_def] >> xsimpl >> 
-     rw[] >> instantiate >> xsimpl)
-  >-(xsimpl) >>
-  xcon >-(
-    xsimpl >> 
-    `nw = 1` by (rw[]) >>
-    fs[] >> rw[] >> fs[insert_atI_def] >>
-    `CHR (ORD c MOD 256) = c` by (fs[CHR_ORD,LESS_MOD,ORD_BOUND]) >>
-    POP_ASSUM (fn x => fs[x]) >>
-    xsimpl) >>
-  xsimpl);
-
-(* TODO: use earlier *)
-val fsupdate_unchanged = Q.store_thm("fsupdate_unchanged",
- `get_file_content fs fd = SOME(content, pos) ==> validFD fd fs ==>
-    fsupdate fs fd 0 pos content = fs`,
-    fs[fsupdate_def,get_file_content_def,validFD_def,IO_fs_component_equality]>>
-    rw[] >> pairarg_tac >> fs[ALIST_FUPDKEY_unchanged] >> rw[]);
+  >-(PURE_REWRITE_TAC[GSYM iobuff_loc_def] >> xsimpl >> 
+     rw[] >> qexists_tac`x` >> xsimpl) >>
+     (* instantiate fails here *)
+  xcon >> fs[IOFS_iobuff_def] >> xsimpl >> rw[] >>
+  fs[CHR_ORD,LESS_MOD,ORD_BOUND] >> qexists_tac`k` >> xsimpl);
 
 val LENGTH_extract_aux = Q.store_thm("LENGTH_extract_aux",
 `!s x y. LENGTH (extract_aux s x y) = y`,
      Induct_on`y` >> fs[extract_aux_def,MIN_DEF]);
+
+val strlen_extract_le = Q.store_thm("strlen_extract_le",
+`!s x y. strlen (extract s x y) <= strlen s - x`,
+  rw[extract_def] >> CASE_TAC >> fs[LENGTH_extract_aux]);
+
+val extract_aux_DROP = Q.store_thm("extract_aux_DROP",
+  `!s k. extract_aux (strlit s) k (LENGTH s - k) = DROP k s`,
+  rw[] >> `?n. STRLEN s - k = n` by fs[] >>
+  FIRST_X_ASSUM MP_TAC >> qid_spec_tac`s` >> qid_spec_tac`k` >>
+  induct_on`n` >> fs[extract_aux_def,STRLEN_DEF,DROP_EL_CONS] >>
+  rw[] >> fs[extract_aux_def,DROP_LENGTH_TOO_LONG] >>
+  (* simplify *)
+  FIRST_X_ASSUM MP_TAC >> PURE_REWRITE_TAC [Once (GSYM SUB_EQ_0)] >>
+  strip_tac >> FIRST_X_ASSUM (fn x => PURE_REWRITE_TAC[x]) >>
+  fs[extract_aux_def])
+
+val extract_aux_eq = Q.store_thm("extract_aux_eq",
+  `!n s. n = LENGTH s ==>
+   extract_aux (strlit s) 0 n = s`,
+  rw[] >> ASSUME_TAC(Q.SPECL[`s`,`0`] extract_aux_DROP) >> fs[]);
+
+val extract_aux_add_r = Q.store_thm("extract_aux_add_r",
+  `!n1 n2 s i. extract_aux s i (n1 + n2) = 
+                extract_aux s i n1 ++ extract_aux s (i+n1) n2`,
+  induct_on`n1` >- fs[extract_aux_def] >>
+  rw[] >> fs[GSYM ADD_SUC,extract_aux_def] >> fs[ADD1]);
+
+val extract_aux_eq = Q.store_thm("extract_aux_eq",
+  `!s n. n = LENGTH s ==>
+   extract_aux (strlit s) 0 n =s`,
+  rw[] >> ASSUME_TAC(Q.SPECL[`s`,`0`] extract_aux_DROP) >> fs[]);
+
+val extract_aux_TAKE = Q.store_thm("extract_aux_TAKE",
+  `!s. n <= LENGTH s ==>
+     extract_aux (strlit s) 0 n = TAKE n s`,
+  rw[] >>
+  sg`extract_aux (strlit s) 0 n ++ extract_aux (strlit s) n (LENGTH s - n)  = 
+     TAKE n s ++ DROP n s`
+  >-(fs[TAKE_DROP, GSYM extract_aux_add_r] >>
+     ASSUME_TAC(Q.SPECL[`n`,`STRLEN s - n`,`strlit s`,`0`]extract_aux_add_r) >>
+     rfs[] >> fs[extract_aux_eq]) >>
+  FIRST_X_ASSUM MP_TAC >> PURE_REWRITE_TAC[extract_aux_DROP] >> rw[]);
 
 val write_string_spec = Q.store_thm("write_string_spec",
   `!s (fd :word8) fdv sv fs content pos. 
@@ -531,95 +623,89 @@ val write_string_spec = Q.store_thm("write_string_spec",
     liveFS fs ⇒ w2n fd < 255 ⇒  wfFS fs ⇒
     (get_file_content fs (w2n fd) = SOME(content, pos)) ⇒
     app (p:'ffi ffi_proj) ^(fetch_v "IO.write_string" (basis_st())) [fdv; sv]
-    (IOFS fs * IOFS_buff257)  
-    (POSTv uv. &(UNIT_TYPE () uv) * IOFS_buff257 * 
+    (IOFS fs * IOFS_iobuff)  
+    (POSTv uv. &(UNIT_TYPE () uv) * IOFS_iobuff * 
        SEP_EXISTS k. IOFS (fsupdate fs (w2n fd) k (pos + (strlen s))
                                     (insert_atI (explode s) pos content)))`,
   strip_tac >>
   `?n. strlen s <= n` by (qexists_tac`strlen s` >> fs[]) >>
   FIRST_X_ASSUM MP_TAC >> qid_spec_tac`s` >>
   Induct_on`n` >>
-  xcf "IO.write_string" (basis_st()) >> fs[IOFS_buff257_def] >>
+  xcf "IO.write_string" (basis_st()) >> fs[IOFS_iobuff_def] >>
   xpull >> rename [`W8ARRAY _ buff`] >>
   Cases_on `buff` >> fs[] >> qmatch_goalsub_abbrev_tac`h1 :: t` >>
-  Cases_on `t` >> fs[] >> qmatch_goalsub_abbrev_tac`h1 :: h2 :: rest` >>
+  Cases_on `t` >> fs[] >> qmatch_goalsub_abbrev_tac`h1 :: h2 :: rest'` >>
+  Cases_on `rest'` >> fs[] >> qmatch_goalsub_abbrev_tac`h1::h2::h3::rest` >>
   (xlet_auto >- xsimpl) >>
   (xif >-(xcon >> xsimpl >> qexists_tac`0` >>
          fs[fsupdate_unchanged,insert_atI_NIL] >> xsimpl))
   >-(cases_on`s` >> fs[strlen_def]) >>
   fs[insert_atI_def] >>
-  sg`STRLEN (explode (substring s 0 254)) + 2 ≤ 257`
+  sg`STRLEN (explode (substring s 0 255)) + 3 ≤ 258`
   >- (fs[LENGTH_explode,substring_def] >> CASE_TAC >>
       fs[substring_def,LENGTH_extract_aux,MIN_DEF]) >>
-  NTAC 5 (xlet_auto >- xsimpl) >>
-  fs[insert_atI_def] >> PURE_REWRITE_TAC[GSYM buff257_loc_def] >>
+  NTAC 4 (xlet_auto >- xsimpl) >>
+  fs[insert_atI_def] >> PURE_REWRITE_TAC[GSYM iobuff_loc_def] >>
   xlet_auto >> xsimpl
-  >-(PURE_REWRITE_TAC[GSYM buff257_loc_def] >> xsimpl >>
+  >-(PURE_REWRITE_TAC[GSYM iobuff_loc_def] >> xsimpl >>
      rw[] >> cases_on`s` >> cases_on`s'` >>
      fs[substring_def,LENGTH_extract_aux,implode_def,strlen_def,MIN_DEF] >>
-     instantiate >> xsimpl) >>
+     qexists_tac`x` >> xsimpl) >> 
+     (* instantiate fails here *)
   xlet_auto >-(xcon >> xsimpl) >>
   sg`OPTION_TYPE NUM NONE (Conv (SOME ("NONE",TypeId (Short "option"))) [])`
   >- fs[OPTION_TYPE_def] >>
   xlet_auto >- xsimpl >>
-  sg`strlen (extract s nw NONE) <= n`
-  >-(fs[extract_def] >> CASE_TAC >> fs[LENGTH_extract_aux]) >>
   qmatch_goalsub_abbrev_tac`fsupdate fs _ _ pos' content'` >>
   qmatch_goalsub_abbrev_tac`IOFS fs'` >>
-  xapp >> xsimpl >>
+  xapp >> fs[IOFS_iobuff_def] >> xsimpl >>
   CONV_TAC(RESORT_EXISTS_CONV List.rev) >>
-  map_every qexists_tac [`content'`,`fd`,`fs'`,`pos'`,`extract s nw NONE`] >>
-  xsimpl >> 
+  map_every qexists_tac [`content'`,`fd`,`fs'`,`pos'`] >>
+  instantiate >> xsimpl >>
   `strlen s <> 0` by (cases_on`s` >> cases_on`s'` >> fs[])>>
   fs[get_file_content_def] >> pairarg_tac >> rw[] >>
   fs[Abbr`fs'`,Abbr`pos'`,Abbr`content'`,liveFS_def,
-     fsupdate_def,LDROP_1, wfFS_fsupdate,validFD_def,always_DROP,extract_def,
-     LENGTH_extract_aux,ALIST_FUPDKEY_ALOOKUP] >>
-  qexists_tac`x' + (Lnext_pos fs.numchars +1)` >> fs[insert_atI_def] >>
+     fsupdate_def,LDROP_1, wfFS_fsupdate,validFD_def,always_DROP,
+     LENGTH_extract_aux,ALIST_FUPDKEY_ALOOKUP,extract_def,strlen_extract_le,
+     substring_def,LENGTH_extract_aux,MIN_DEF] >> xsimpl
+  >-(CASE_TAC >> CASE_TAC >> fs[implode_def,LENGTH_extract_aux]) >>
+  qexists_tac`x' + k` >> fs[insert_atI_def] >>
   qmatch_abbrev_tac`IOFS fs1 ==>> IOFS fs2 * GC` >>
-  `fs1 = fs2` suffices_by xsimpl >> 
-  fs[Abbr`fs1`,Abbr`fs2`] >>
-  `nw <= strlen s` by fs[substring_def, LENGTH_extract_aux] >>
+  `fs1 = fs2` suffices_by xsimpl >> fs[Abbr`fs1`,Abbr`fs2`] >>
+  cases_on`s` >>
   rw[] >> fs[ALIST_FUPDKEY_o,LENGTH_extract_aux,MAP_MAP_o,CHR_w2n_n2w_ORD,
-             LENGTH_explode] >> 
-  TRY(MATCH_MP_TAC ALIST_FUPDKEY_eq >> fs[LENGTH_TAKE])
-  >-(`nw = strlen s` by fs[] >>
-     sg`nw <= STRLEN (explode (substring s 0 254))` 
-     >- fs[LENGTH_explode,LENGTH_extract_aux,substring_def] >>
-     sg`strlen s <= 255`
-     >- fs[LENGTH_explode,LENGTH_extract_aux,substring_def] >>
-     fs[TAKE_APPEND1,TAKE_LENGTH_TOO_LONG]>>
-     fs[LENGTH_explode,LENGTH_extract_aux,substring_def,MIN_DEF] >>
-     CASE_TAC >>
-    (* TODO lemma *)
-     cheat)
-  >-(`nw < strlen s` by fs[] >> cheat)
-  >-(
-      sg`!k. ?v. LDROP k fs.numchars = SOME v`
-      >-(imp_res_tac always_NOT_LFINITE >>
-         fs[LFINITE_DROP,NOT_LFINITE_DROP,always_NOT_LFINITE]) >>
-  cheat)
-);
+             LENGTH_explode,LENGTH_TAKE_EQ, LENGTH_extract_aux,strlen_def,
+             TAKE_APPEND,TAKE_LENGTH_TOO_LONG,extract_aux_eq,extract_aux_DROP] >> 
+  TRY(MATCH_MP_TAC ALIST_FUPDKEY_eq >> fs[LENGTH_TAKE]) 
+  >-(`STRLEN s' = 255` by fs[] >> fs[DROP_LENGTH_TOO_LONG])
+  >-(`255 <= STRLEN s'` by fs[] >> fs[extract_aux_TAKE] >>
+     fs[DROP_LENGTH_TOO_LONG,LENGTH_TAKE_EQ,LENGTH_extract_aux,LENGTH_APPEND] >>
+     CASE_TAC >> fs[DROP_APPEND,DROP_LENGTH_TOO_LONG,DROP_DROP_T,LENGTH_TAKE_EQ])
+  >-(fs[LDROP_ADD] >> CASE_TAC >> fs[] >>
+     sg`?v. LDROP k fs.numchars = SOME v`
+     >-(imp_res_tac always_NOT_LFINITE >>
+        fs[LFINITE_DROP,NOT_LFINITE_DROP,always_NOT_LFINITE]) >>
+     fs[]));
 
 val read_spec = Q.store_thm("read_spec",
   `validFD (w2n fd) fs ⇒ w2n fd < 255 ⇒
    WORD (fd:word8) fdv ⇒ WORD (n:word8) nv ⇒ 
-   LENGTH rest = 255 ⇒  w2n n <= 255 ⇒ 
+   LENGTH rest = 256 ⇒  w2n n <= 255 ⇒ 
    wfFS fs ⇒  get_file_content fs (w2n fd) = SOME(content, pos) ⇒
    app (p:'ffi ffi_proj) ^(fetch_v "IO.read" (basis_st())) [fdv;nv]
-   (W8ARRAY buff257_loc (h1 :: h2 :: rest) * IOFS fs)
+   (W8ARRAY iobuff_loc (h1 :: h2 :: rest) * IOFS fs)
    (POSTv uv. 
       &(UNIT_TYPE () uv) * 
       SEP_EXISTS nr. &(nr <= MIN (w2n n) (LENGTH content - pos) /\
                       (nr = 0 ⇔ eof (w2n fd) fs = SOME T ∨ w2n n = 0)) * 
       IOFS (bumpFD (w2n fd) fs nr) *
-      W8ARRAY buff257_loc (0w :: n2w nr :: 
+      W8ARRAY iobuff_loc (0w :: n2w nr :: 
         MAP (n2w o ORD) (TAKE nr (DROP pos content))++DROP nr rest))`,
    xcf "IO.read" (basis_st()) >> 
    NTAC 2 (xlet_auto >- (fs[LUPDATE_def] >> xsimpl)) >>
    simp[LUPDATE_def,EVAL ``LUPDATE rr 1 (zz :: tt)``] >>
    xffi >> xsimpl >>
-   fs[buff257_loc,IOFS_def,IOx_def,fs_ffi_part_def, mk_ffi_next_def] >>
+   fs[iobuff_loc,IOFS_def,IOx_def,fs_ffi_part_def, mk_ffi_next_def] >>
    qmatch_goalsub_abbrev_tac`IO st f ns` >>
    CONV_TAC(RESORT_EXISTS_CONV List.rev) >>
    map_every qexists_tac[`ns`,`f`] >>
@@ -641,20 +727,20 @@ val read_char_spec = Q.store_thm("read_char_spec",
     WORD fd fdv ⇒ validFD (w2n fd) fs ⇒ w2n fd < 255 ⇒
     wfFS fs ⇒  get_file_content fs (w2n fd) = SOME(content, pos) ⇒
     app (p:'ffi ffi_proj) ^(fetch_v "IO.read_char" (basis_st())) [fdv]
-    (IOFS fs * IOFS_buff257) 
+    (IOFS fs * IOFS_iobuff) 
     (POST (\cv. &(WORD (n2w (ORD (EL pos content)):word8) cv /\
                 eof (w2n fd) fs = SOME F) *
-                IOFS_buff257 * IOFS (bumpFD (w2n fd) fs 1))
+                IOFS_iobuff * IOFS (bumpFD (w2n fd) fs 1))
           (\e.  &(EndOfFile_exn e /\ eof (w2n fd) fs = SOME T) *
-                IOFS_buff257 * IOFS(bumpFD (w2n fd) fs 0)))`,
-  xcf "IO.read_char" (basis_st()) >> fs[IOFS_buff257_def] >> 
+                IOFS_iobuff * IOFS(bumpFD (w2n fd) fs 0)))`,
+  xcf "IO.read_char" (basis_st()) >> fs[IOFS_iobuff_def] >> 
   xpull >> rename [`W8ARRAY _ bdef`] >>
   Cases_on `bdef` >> fs[] >> qmatch_goalsub_abbrev_tac`h1 :: t` >>
   Cases_on `t` >> fs[] >> qmatch_goalsub_abbrev_tac`h1 :: h2 :: t'` >>
   Cases_on `t'` >> fs[] >> qmatch_goalsub_abbrev_tac`h1 :: h2 :: h3 :: rest` >>
   xlet_auto >- xsimpl >>
-  PURE_REWRITE_TAC[GSYM buff257_loc_def] >>
-  xlet_auto >-(fs[buff257_loc_def] >> xsimpl >> rw[] >> instantiate >> xsimpl)>>
+  PURE_REWRITE_TAC[GSYM iobuff_loc_def] >>
+  xlet_auto >-(fs[iobuff_loc_def] >> xsimpl >> rw[] >> instantiate >> xsimpl)>>
   NTAC 3 (xlet_auto >- xsimpl) >>
   xif >> instantiate >>
   NTAC 3 (xlet_auto >- xsimpl) >>
@@ -665,5 +751,4 @@ val read_char_spec = Q.store_thm("read_char_spec",
   fs[take1_drop,eof_def,get_file_content_def] >> pairarg_tac >> fs[]);
  
 val _ = export_theory();
-
 
